Solve Q1.4 after rewriting a lot of things
Signed-off-by: Nicolas Iooss <nicolas.iooss_git@polytechnique.org>

lambda_calcul.v
@@ -15,47 +15,79 @@ Definition l_id: lterm := Lambda (Var 0)
 .
 
 (* Predicate: every free variable has an index below n *)
-Fixpoint freevars_below (n: nat) (t: lterm) : Prop :=
+Fixpoint fr_below (n: nat) (t: lterm) : Prop :=
   match t with
     | Var x => x < n
-    | Lambda u => freevars_below (S n) u
-    | Apply u v => (freevars_below n u) /\ (freevars_below n v)
+    | Lambda u => fr_below (S n) u
+    | Apply u v => (fr_below n u) /\ (fr_below n v)
   end
 .
 
 (* Closed term *)
 Definition closed (t: lterm) : Prop :=
-  freevars_below 0 t
+  fr_below 0 t
 .
 
-(* freevars_below is still True when n increases *)
-Theorem freevars_below_S:
+(* fr_below is still True when n increases *)
+Theorem fr_below_S:
   forall (t: lterm) (n: nat),
-  freevars_below n t -> freevars_below (S n) t.
+  fr_below n t -> fr_below (S n) t.
 Proof.
   induction t; simpl.
-    intros n0 H. apply lt_S. trivial.
-    intros n H. apply (IHt (S n)). trivial.
+    auto with arith.
+    intros n H. apply (IHt (S n)); trivial.
     intros n H. apply conj.
-      apply IHt1. apply H.
-      apply IHt2. apply H.
+      apply IHt1; apply H.
+      apply IHt2; apply H.
 Save.
-Theorem freevars_below_incr:
+
+Theorem fr_below_incr:
   forall (t: lterm) (n m: nat),
-  freevars_below n t /\ n <= m -> freevars_below m t.
+  fr_below n t /\ n <= m -> fr_below m t.
 Proof.
   intros t n; induction m; intro H; destruct H.
     cut (O = n).
-      intro H1. rewrite H1. trivial.
-      apply (le_n_0_eq n). trivial.
+      intro H1; rewrite H1; trivial.
+      auto with arith.
 
-    cut (n < S m \/ n = S m). (*(n = S m) \/ (n <= m)*)
-      intro H1. destruct H1.
-        apply (freevars_below_S t m). apply IHm.
-        apply conj. trivial. apply (lt_n_Sm_le n m). trivial.
+    cut (n < S m \/ n = S m).
+      intro H1; destruct H1.
+        apply (fr_below_S t m). apply IHm.
+        apply conj; trivial; auto with arith.
 
-        rewrite <- H1. trivial.
-      apply (le_lt_or_eq n (S m)). trivial.
+        rewrite <- H1; trivial.
+      apply (le_lt_or_eq n (S m)); trivial.
+Save.
+
+(* forall u in ul, fr_below n u *)
+Fixpoint fr_below_list (n: nat) (ul: list lterm) : Prop :=
+  match ul with
+    | nil => True
+    | u :: l => (fr_below n u) /\ (fr_below_list n l)
+  end
+.
+
+Lemma fr_below_list_forall:
+  forall (n: nat) (ul: list lterm),
+  fr_below_list n ul -> (forall u: lterm, In u ul -> fr_below n u).
+Proof.
+  intro n; induction ul; simpl; intros H u H0.
+    contradict H0.
+    destruct H. destruct H0.
+      rewrite <- H0; trivial.
+      apply IHul; trivial.
+Save.
+
+(* fr_below_list is still True when n increases *)
+Theorem fr_below_list_S:
+  forall (n: nat) (ul: list lterm),
+  fr_below_list n ul -> fr_below_list (S n) ul.
+Proof.
+  induction ul; simpl; trivial.
+    intro H; destruct H.
+    split.
+      apply fr_below_S; trivial.
+      apply IHul; trivial.
 Save.
 
 (*
@@ -65,103 +97,285 @@ Save.
  * (Var 1)[0 <- u] = Var 1
  * (Lambda t)[0 <- u] = Lambda (t[1 <- u])
  *)
-Fixpoint substitute (t: lterm) (x: nat) (u: lterm) : lterm :=
+Fixpoint subst (t: lterm) (x: nat) (u: lterm) : lterm :=
   match t with
     | Var y => if beq_nat x y then u else t
-    | Lambda t0 => Lambda (substitute t0 (S x) u)
-    | Apply t0 u0 => Apply (substitute t0 x u) (substitute u0 x u)
+    | Lambda t0 => Lambda (subst t0 (S x) u)
+    | Apply t0 u0 => Apply (subst t0 x u) (subst u0 x u)
   end
 .
 
 (* Substitution on a free variable does nothing *)
-Lemma substitute_freevars_eq:
-  forall (t: lterm) (n: nat) (x: nat) (u: lterm),
-  ((freevars_below n t) /\ (x >= n)) -> (substitute t x u) = t.
+Lemma substitute_freevar_eq:
+  forall (t: lterm) (x: nat) (u: lterm), fr_below x t -> subst t x u = t.
 Proof.
-  induction t.
-    intros n0 x u H. simpl.
-    destruct H.
+  induction t; simpl; intros x u H.
     assert (beq_nat x n = false).
       rewrite (beq_nat_false_iff x n).
-      apply lt_neq_sym.
-      apply (lt_le_trans n n0 x); trivial.
-    rewrite H1. trivial.
+      apply lt_neq_sym; trivial.
+    rewrite H0; trivial.
 
-    intros n x u H. simpl. 
-    rewrite (IHt (S n) (S x) u); trivial.
-    apply conj. apply H. apply (le_n_S n x). apply H.
+    rewrite (IHt (S x) u); trivial.
 
-    intros n x u H. simpl. 
-    rewrite (IHt1 n x u). rewrite (IHt2 n x u). trivial.
-    apply conj; apply H.
-    apply conj; apply H.
+    destruct H.
+    rewrite (IHt1 x u); trivial.
+    rewrite (IHt2 x u); trivial.
 Save.
 
 (* Substitution on a closed term does nothing *)
 Theorem substitute_closed_eq:
-  forall (t: lterm) (x: nat) (u: lterm), closed t -> (substitute t x u) = t.
+  forall (t: lterm) (x: nat) (u: lterm), closed t -> subst t x u = t.
 Proof.
   intros t x u H.
-  apply (substitute_freevars_eq t 0 x u).
+  apply (substitute_freevar_eq t x u).
+  apply (fr_below_incr t 0 x).
   apply conj.
-  apply H.
-  apply le_0_n.
+    apply H.
+    apply le_0_n.
 Save.
 
 (* Substitution of variable x in a list i->u0, i+1->u1, i+2->u2, ...
  * Return d by default
  *)
-Fixpoint substitute_var_list (x i: nat) (ul: list lterm) (d: lterm) : lterm :=
+Fixpoint subst_var_list (x i: nat) (ul: list lterm) (d: lterm) : lterm :=
   match ul, i, x with
     | nil, _, _ => d
     | t :: _, O, O => t
-    | _ :: vl, O, S y => substitute_var_list y O vl d
+    | _ :: vl, O, S y => subst_var_list y O vl d
     | _ :: _, S _, O => d
-    | _ :: _, S j, S y => substitute_var_list y j ul d
+    | _ :: _, S j, S y => subst_var_list y j ul d
   end
 .
 
-(* Substitution with a list of terms i->u0, i+1->u1, i+2->u2, ... *)
-Fixpoint substitute_list (t: lterm) (i: nat) (u: list lterm) : lterm :=
-  match t with
-    | Var x =>  substitute_var_list x i u (Var x)
-    | Lambda t0 => Lambda (substitute_list t0 (S i) u)
-    | Apply t0 u0 => Apply (substitute_list t0 i u) (substitute_list u0 i u)
-  end
-.
-Theorem substitute_list_empty:
-  forall (t: lterm) (i: nat), substitute_list t i nil = t.
+Lemma substitute_vl_nil:
+  forall (n x: nat) (d: lterm), subst_var_list n x nil d = d.
 Proof.
-  induction t; intro i; simpl.
-    induction n; induction i; trivial.
-    rewrite (IHt (S i)). trivial.
-    rewrite IHt1; rewrite IHt2. trivial.
+  induction n; trivial.
 Save.
+Hint Resolve substitute_vl_nil : substitute.
 
-Lemma substitute_var_list_eq:
-  (* i = n + a + 1 *)
+Lemma substitute_vl_eq:
+  forall (n: nat) (u: lterm) (ul: list lterm) (d: lterm),
+  subst_var_list n n (u :: ul) d = u.
+Proof.
+  induction n; simpl; trivial.
+Save.
+Hint Resolve substitute_vl_eq : substitute.
+
+(* (Var n)[(n + a + 1) <- ul_0, ul_1, ...] = (Var n), a is called "diff" *)
+Lemma substitute_vl_lt_with_diff:
   forall (n a: nat) (ul: list lterm) (d: lterm),
-    substitute_var_list n (n + 1 + a) ul d = d.
+  subst_var_list n (n + 1 + a) ul d = d.
 Proof.
   induction n; induction a; induction ul; intro d; simpl; trivial.
 Save.
 
+Lemma substitute_vl_lt:
+  forall (x i: nat) (ul: list lterm) (d: lterm),
+  x < i -> subst_var_list x i ul d = d.
+Proof.
+  intros x i ul d H.
+  cut (i = x + 1 + (i - (x + 1))).
+    intro H0; rewrite H0. auto.
+    apply (substitute_vl_lt_with_diff x (i - (x + 1)) ul d).
+
+    apply (le_plus_minus (x + 1) i).
+    rewrite <- (plus_Sn x).
+    apply (lt_le_S x i).
+    apply H.
+Save.
+Hint Immediate substitute_vl_lt : substitute.
+
+(* The proof of this lemme uses an induction on i which impacts the order of parameters *)
+Lemma substitute_vl_gt_prooforder:
+  forall (i x: nat) (u: lterm) (ul: list lterm) (d: lterm),
+  x > i -> subst_var_list x i (u :: ul) d = subst_var_list x (S i) ul d.
+Proof.
+  induction i; intros x u ul d H; simpl; cut (x = S (pred x)).
+    intro H0; rewrite H0.
+    induction ul; simpl; auto with substitute.
+
+    apply (S_pred x 0); trivial.
+
+    intro H0; rewrite H0; simpl.
+    rewrite (IHi (pred x) u ul d).
+      induction ul; auto with substitute.
+      auto with arith.
+    apply (S_pred x (S i)); trivial.
+Save.
+
+(* Same as above, change parameters order *)
+Lemma substitute_vl_gt:
+  forall (x i: nat) (u: lterm) (ul: list lterm) (d: lterm),
+  x > i -> subst_var_list x i (u :: ul) d = subst_var_list x (S i) ul d.
+Proof.
+  intros; apply substitute_vl_gt_prooforder; trivial.
+Save.
+Hint Immediate substitute_vl_gt : substitute.
+
+Lemma substitute_vl_ne:
+  forall (x i: nat) (u: lterm) (ul: list lterm) (d: lterm),
+  x <> i -> subst_var_list x i (u :: ul) d = subst_var_list x (S i) ul d.
+Proof.
+  intros x i u ul d H.
+  cut (x < i \/ x > i).
+    intro H0; destruct H0.
+    rewrite (substitute_vl_lt x i (u::ul) d); trivial.
+    rewrite (substitute_vl_lt x (S i) ul d); auto with arith.
+    apply (substitute_vl_gt x i u ul d); trivial.
+    apply (nat_total_order x i); trivial.
+Save.
+
+Lemma substitue_vl_nth_with_diff:
+  forall (n: nat) (ul: list lterm) (i: nat) (d: lterm),
+  subst_var_list (i + n) i ul d = nth n ul d.
+Proof.
+  induction n; induction ul; intros i d; simpl.
+    auto with substitute.
+    rewrite <- (plus_n_O i). apply (substitute_vl_eq i a ul d).
+    auto with substitute.
+    rewrite (substitute_vl_gt (i + S n) i a ul d).
+      rewrite <- (plus_n_Sm i n).
+      rewrite <- (plus_Sn_m i n).
+      apply (IHn ul (S i) d).
+
+      rewrite <- (plus_n_Sm i n).
+      apply (le_lt_n_Sm i (i + n)).
+      apply (le_plus_l i n).
+Save.
+
+Lemma substitute_vl_nth:
+  forall (x i: nat) (ul: list lterm) (d: lterm),
+  i <= x -> subst_var_list x i ul d = nth (x - i) ul d.
+Proof.
+  intros x i ul d H.
+  cut (x = i + (x - i)).
+    intro H0; rewrite H0.
+    rewrite (substitue_vl_nth_with_diff (x - i) ul i d).
+    rewrite <- H0; trivial.
+    auto with arith.
+Save.
+
+Lemma substitute_vl_in:
+  forall (x i: nat) (ul: list lterm) (d: lterm),
+  i <= x < i + length ul -> In (subst_var_list x i ul d) ul.
+Proof.
+  intros x i ul d H; destruct H.
+  rewrite (substitute_vl_nth x i ul d); trivial.
+  apply (nth_In ul d).
+  apply (plus_lt_reg_l (x - i) (length ul) i).
+  rewrite <- (le_plus_minus i x); trivial.
+Save.
+
+Lemma substitute_vl_gt_overflow:
+  forall (x i: nat) (ul: list lterm) (d: lterm),
+  x >= i + length ul -> subst_var_list x i ul d = d.
+Proof.
+  intros x i ul d H.
+  cut (x >= i).
+    intro H0.
+    rewrite (substitute_vl_nth x i ul d); trivial.
+    apply (nth_overflow ul d).
+    apply (plus_le_reg_l (length ul) (x - i) i).
+    rewrite <- (le_plus_minus i x); trivial.
+    eauto with arith.
+Save.
+
+Lemma substitute_vl_values:
+  forall (x i: nat) (ul: list lterm) (d: lterm),
+  subst_var_list x i ul d = d \/ In (subst_var_list x i ul d) ul.
+Proof.
+  intros x i ul d.
+  cut (i + length ul <= x \/ x < i + length ul).
+    intro H; destruct H.
+      apply or_introl. apply substitute_vl_gt_overflow; trivial.
+      cut (i <= x \/ x < i).
+        intro H0; destruct H0.
+          apply or_intror. apply substitute_vl_in; auto.
+          apply or_introl. apply substitute_vl_lt; trivial.
+
+        apply le_or_lt.
+    apply le_or_lt.
+Save.
+
+(* Substitution with a list of terms i->u0, i+1->u1, i+2->u2, ... *)
+Fixpoint subst_list (t: lterm) (i: nat) (u: list lterm) : lterm :=
+  match t with
+    | Var x =>  subst_var_list x i u (Var x)
+    | Lambda t0 => Lambda (subst_list t0 (S i) u)
+    | Apply t0 u0 => Apply (subst_list t0 i u) (subst_list u0 i u)
+  end
+.
+
+Theorem substitute_list_empty:
+  forall (t: lterm) (i: nat), subst_list t i nil = t.
+Proof.
+  induction t; intro i; simpl.
+    induction n; induction i; trivial.
+    rewrite (IHt (S i)); trivial.
+    rewrite IHt1; rewrite IHt2; trivial.
+Save.
+
 Theorem substitute_singlelist_free_eq:
   forall (t: lterm) (i: nat) (u: lterm),
-  freevars_below i t -> substitute_list t i (u :: nil) = t.
+  fr_below i t -> subst_list t i (u :: nil) = t.
 Proof.
   induction t; simpl; intros i u H; simpl.
-    rewrite (le_plus_minus (n + 1) i).
-    rewrite (minus_plus_simpl i n 1).
-    apply (substitute_var_list_eq n (i - n - 1) (u :: nil) (Var n)).
-    rewrite <- (plus_n_Sm n O).
-    rewrite <- (plus_n_O n).
-    apply (lt_le_S n i).
-    trivial.
-
+    auto with substitute.
     rewrite (IHt (S i) u); trivial.
-
     destruct H.
     rewrite (IHt1 i u); trivial.
     rewrite (IHt2 i u); trivial.
 Save.
+
+
+Theorem substitute_list_cons_free_eq:
+  forall (t: lterm) (ul: list lterm) (i: nat) (u: lterm),
+  fr_below_list i ul ->
+    subst_list t i (u :: ul) = subst_list (subst_list t (S i) ul) i (u :: nil).
+Proof.
+  induction t; simpl.
+    induction ul; simpl; intros i u H.
+      induction i; induction n; trivial.
+      destruct H.
+      cut (n = i \/ n <> i).
+        intro H1; destruct H1.
+          (* n = i *)
+          rewrite <- H1.
+          rewrite (substitute_vl_eq n u (a :: ul) (Var n)).
+          rewrite (substitute_vl_lt n (S n) (a :: ul) (Var n)); auto with arith.
+          simpl.
+          auto with substitute.
+          (* n <> i *)
+          rewrite (substitute_vl_ne n i u (a :: ul) (Var n)); trivial.
+          cut (subst_var_list n (S i) (a :: ul) (Var n) = Var n \/
+               In (subst_var_list n (S i) (a :: ul) (Var n)) (a :: ul)).
+            intro H2; destruct H2.
+              rewrite H2; simpl.
+              rewrite substitute_vl_ne; trivial.
+              rewrite substitute_vl_nil; trivial.
+
+              rewrite (substitute_singlelist_free_eq
+                       (subst_var_list n (S i) (a :: ul) (Var n)) i u); trivial.
+
+              cut (a = subst_var_list n (S i) (a :: ul) (Var n) \/
+                   In (subst_var_list n (S i) (a :: ul) (Var n)) ul).
+                intro H3; destruct H3.
+                  rewrite <- H3; trivial.
+                  apply (fr_below_list_forall i ul); trivial.
+                apply in_inv; trivial.
+
+            apply (substitute_vl_values n (S i) (a :: ul) (Var n)).
+        apply neq_or_eq.
+
+    (* Lambda *)
+    intros ul i u H.
+      rewrite IHt; trivial.
+      apply fr_below_list_S; trivial.
+
+    (* Apply *)
+    intros ul i u H.
+      rewrite IHt1; trivial.
+      rewrite IHt2; trivial.
+Save.
+
