Arith_ext.v
@@ -18,3 +18,43 @@ Theorem minus_plus_simpl:
 Proof.
   induction n; induction m; induction p; simpl; trivial.
 Save.
+
+Theorem plus_Sn:
+  forall n: nat, S n = n + 1.
+Proof.
+  intro n. rewrite (plus_comm n 1). trivial.
+Save.
+
+Theorem lt_S_lt_or_eq:
+  forall (n m: nat), n < S m -> n < m \/ n = m.
+Proof.
+  intros n m H.
+  apply (le_lt_or_eq n m).
+  apply (lt_n_Sm_le n m).
+  apply H.
+Save.
+
+Theorem le_exists_diff:
+  forall (n m: nat), n <= m -> exists d: nat, m = n + d.
+Proof.
+  intros n m H.
+  exists (m - n).
+  apply (le_plus_minus n m).
+  apply H.
+Save.
+
+(* Let's proove trivial things *)
+Theorem neq_or_eq:
+  forall (n m: nat), n = m \/ n <> m.
+Proof.
+  intros n m.
+  cut (n <= m \/ m < n).
+    intro H; destruct H.
+      cut (n < m \/ n = m).
+        intro H0; destruct H0.
+          apply or_intror. apply lt_neq; trivial.
+          apply or_introl; trivial.
+        apply (le_lt_or_eq n m); trivial.
+      apply or_intror. apply lt_neq_sym; trivial.
+    apply le_or_lt.
+Save.
